src/lib.lean
@@ -1,6 +1,6 @@
 import tactic data.equiv.encodable.basic
 
-universe u
+universes u v
 
 attribute [instance, priority 0] classical.prop_decidable
 
@@ -11,12 +11,12 @@ inductive dvector (α : Type u) : ℕ → Type u
 notation a :: b  := dvector.cons a b
 
 namespace dvector
-variables {α : Type u}
+variables {α : Type u} {β : Type v}
 
 @[simp] def unary (a : α) : dvector α 1 := a :: nil
 
 @[simp] def extract : dvector α 1 → α
-| (a :: nil) := a
+| (a :: _) := a
 
 @[simp] lemma extract_nil : ∀ (v : dvector α 1), v.extract :: nil = v
 | (a :: nil) := rfl
@@ -24,6 +24,14 @@ variables {α : Type u}
 @[simp] protected def append : ∀ {n}, dvector α n → ∀ {m}, dvector α m → dvector α (m + n)
 | _ nil      _ l := l
 | _ (a :: l) _ k := a :: (append l k)
+
+def filter (f : α → β) : ∀ {n}, dvector α n → dvector β n
+| 0     _         := dvector.nil
+| (n+1) (a :: as) := f a :: filter as
+
+@[simp] def app {C : Π i : α, Type v} (a) : ∀ {n}, dvector (Π i, C i) n → dvector (C a) n
+| 0     _         := dvector.nil
+| (n+1) (f :: fs) := f a :: app fs
 
 end dvector
 
@@ -38,3 +46,67 @@ lemma idecode_surj : function.surjective (idecode α) := surjective_decode_iget 
 by simp[idecode, encodek]
 
 end encodable
+
+namespace setoid
+
+@[simp] def vec_r {α : Type u} [s : setoid α] : ∀ {n}, dvector α n → dvector α n → Prop
+| 0     _         _         := true
+| (n+1) (a :: as) (b :: bs) := a ≈ b ∧ vec_r as bs
+
+infix ` ≋ `:80 := vec_r
+
+@[simp] lemma vec_r_refl {α : Type u} [s : setoid α] {n} (v : dvector α n) : vec_r v v
+:= by induction v; simp*
+
+lemma vec_r_symm {α : Type u} [s : setoid α] : ∀ {n} {v w : dvector α n}, vec_r v w → vec_r w v
+| 0 _ _ := by simp
+| (n+1) (a :: as) (b :: bs) := by { simp, refine λ e h, ⟨setoid.symm e, vec_r_symm h⟩ }
+
+lemma vec_r_trans {α : Type u} [s : setoid α] : ∀ {n} {a b c : dvector α n}, vec_r a b → vec_r b c → vec_r a c
+| 0 _ _ _ := by simp
+| (n+1) (a :: as) (b :: bs) (c :: cs) := by { simp, refine λ e₁ h₁ e₂ h₂, ⟨setoid.trans e₁ e₂, vec_r_trans h₁ h₂⟩ }
+
+lemma vec_r_equiv {α : Type u} [s : setoid α] {n} : equivalence (@vec_r α s n) := ⟨vec_r_refl, λ _ _, vec_r_symm, λ _ _ _, vec_r_trans⟩
+
+def vec {α : Type u} (s : setoid α) (n) : setoid (dvector α n) := ⟨@vec_r α s n, vec_r_equiv⟩
+
+@[simp] lemma vec_r_simp_nil {α : Type*} [s : setoid α] :
+  (dvector.nil : dvector α 0) ≋ dvector.nil := by simp[has_equiv.equiv]
+
+@[simp] lemma vec_r_simp_cons {α : Type*} [s : setoid α] {n} {a b : α} {as bs : dvector α n} :
+  (a :: as) ≋ (b :: bs) ↔ a ≈ b ∧ as ≋ bs := by { simp, }
+
+@[simp] lemma vec_r_equiv_equiv {α : Type*} [s : setoid α] {n} {a b : dvector α n} :
+  @setoid.r _ (s.vec n) a b ↔ a ≋ b := iff.rfl
+
+end setoid
+
+namespace quotient
+universes u_a u_b u_c
+variables {α : Type u_a} {β : Sort u_b} {φ : Sort u_c}
+
+def mk_vec (s : setoid α) (n : ℕ) : Type* := quotient (s.vec n)
+
+def extract (s : setoid α) : quotient (s.vec 1) → quotient s :=
+λ q, @quotient.lift_on _ _ (s.vec 1) q (λ v, ⟦dvector.extract v⟧) $ λ a b,
+by { cases a with _ a n, cases n, cases b with _ b n, cases n, simp[has_equiv.equiv] }
+
+def cons_aux (s : setoid α) (a : α) {n} : quotient (s.vec n) → quotient (s.vec (n+1)) :=
+λ q, @quotient.lift_on _ _ (s.vec n) q (λ v, @quotient.mk _ (s.vec (n+1)) (a :: v)) $
+λ as bs, by { simp, refine λ h, ⟨by refl, h⟩ }
+
+def cons (s : setoid α) {n} : quotient s → quotient (s.vec n) → quotient (s.vec (n+1)) :=
+λ q v, @quotient.lift_on _ _ s q (λ a, cons_aux s a v) $ λ as bs eqn, by { simp[cons_aux],
+  induction v, simp[eqn, has_equiv.equiv], refine eqn, refl }
+
+@[simp] def dvec_to_quo (s : setoid α) : ∀ {n}, dvector (quotient s) n → quotient (s.vec n)
+| 0     _         := @quotient.mk _ (s.vec 0) (dvector.nil : dvector α 0)
+| (n+1) (q :: qs) := cons s q (dvec_to_quo qs)
+
+@[elab_as_eliminator, reducible]
+def lift_on_vec {s : setoid α} {n} (q : dvector (quotient s) n) (f : dvector α n → φ)
+  (c : ∀ a b : dvector α n, (@setoid.vec_r _ s _ a b) → f a = f b) : φ :=
+@quotient.lift_on _ _ (s.vec _) (dvec_to_quo s q) f c
+
+end quotient
+
